Complete the construction of the universal machine for the lambda-calculus.  The UM is defined in recfunsTheory, where I will also put stuff like the s-m-n theorem.  When we've figured out how to represent the standard recursive function requirements (they are of multiple arities in the presentations I've seen, making typing a pain), I'll also show that the recursive constructions are possible in the lambda-calculus.

examples/computability/lambda/churchDBScript.sml
@@ -1188,6 +1188,46 @@ val cis_church_behaviour = store_thm(
   ]);
 
 (* ----------------------------------------------------------------------
+    cforceNum
+   ---------------------------------------------------------------------- *)
+
+val cforce_num_def = Define`
+  cforce_num =
+  LAM "t" (cis_church @@ VAR "t"
+                      @@ (cminus @@ (cdiv @@ (cdbsize @@ VAR "t") @@ church 2)
+                                 @@ church 1)
+                      @@ church 0)
+`;
+
+val FV_cforce_num = Store_thm(
+  "FV_cforce_num",
+  ``FV cforce_num = {}``,
+  SRW_TAC [][EXTENSION, cforce_num_def]);
+
+val cforce_num_equiv0 = brackabs_equiv [] cforce_num_def
+val cforce_num_equiv = brackabs_equiv [B_I_uncond] cforce_num_equiv0
+
+val dbsize_fromTerm = Store_thm(
+  "dbsize_fromTerm",
+  ``∀t. dbsize (fromTerm t) = size t``,
+  HO_MATCH_MP_TAC simple_induction THEN SRW_TAC [][]);
+
+val size_toTerm = save_thm(
+  "size_toTerm",
+  dbsize_fromTerm |> Q.SPEC `toTerm d` |> REWRITE_RULE [fromtoTerm] |> SYM);
+val _ = export_rewrites ["size_toTerm"]
+
+val cforce_num_behaviour = store_thm(
+  "cforce_num_behaviour",
+  ``cforce_num @@ cDB t -n->* church (force_num (toTerm t))``,
+  SIMP_TAC (bsrw_ss()) [cforce_num_equiv, cdbsize_behaviour, cdiv_behaviour,
+                        cminus_behaviour, cis_church_behaviour] THEN
+  Cases_on `is_church (toTerm t)` THENL [
+    ASM_SIMP_TAC (bsrw_ss()) [cB_behaviour, force_num_size],
+    ASM_SIMP_TAC (bsrw_ss()) [force_num_def, cB_behaviour]
+  ]);
+
+(* ----------------------------------------------------------------------
     cciDB : the encoded/computing version of ciDB
    ---------------------------------------------------------------------- *)
 
@@ -1403,9 +1443,10 @@ val cnumdB_behaviour = store_thm(
 
 val cbnfof_body_def = Define`
   cbnfof_body =
-  LAM "f" (LAM "t" (cbnf @@ VAR "t"
-                         @@ VAR "t"
-                         @@ (VAR "f" @@ (cnoreduct @@ VAR "t"))))
+  LAM "c" (LAM "f" (LAM "t"
+    (cbnf @@ VAR "t"
+          @@ (VAR "c" @@ VAR "t")
+          @@ (VAR "f" @@ (cnoreduct @@ VAR "t")))))
 `;
 
 val cbnfof_body_equiv0 = brackabs_equiv [] cbnfof_body_def
@@ -1418,34 +1459,20 @@ val FV_cbnfof_body = Store_thm(
 
 val _ = reveal "Y"
 
-val cbnf_of_def = Define`cbnf_of = Y @@ cbnfof_body`
+
+val cbnf_ofk_def = Define`
+  cbnf_ofk = B @@ Y @@ cbnfof_body
+`;
+val FV_cbnf_ofk = Store_thm(
+  "FV_cbnf_ofk",
+  ``FV cbnf_ofk = {}``,
+  SRW_TAC [][EXTENSION, cbnf_ofk_def]);
+
+val cbnf_of_def = Define`cbnf_of = cbnf_ofk @@ I`
 val FV_cbnf = Store_thm(
   "FV_cbnf",
   ``FV cbnf_of = {}``,
   SRW_TAC [][cbnf_of_def]);
-
-val cbnf_of_lemma = prove(
-  ``∀t. (OWHILE ((~) o bnf) (THE o noreduct) t0 = SOME t) ⇒
-        Y @@ cbnfof_body @@ cDB (fromTerm t0) ==
-          Y @@ cbnfof_body @@ cDB (fromTerm t)``,
-  HO_MATCH_MP_TAC whileTheory.OWHILE_INV_IND THEN SRW_TAC [][] THEN
-  ASM_SIMP_TAC (bsrw_ss()) [] THEN
-  ASM_SIMP_TAC (bsrw_ss()) [Once chap2Theory.lameq_Y] THEN
-  ASM_SIMP_TAC (bsrw_ss()) [cbnfof_body_equiv, cbnf_behaviour,
-                            cnoreduct_behaviour, cB_behaviour]);
-
-val cbnf_of_works1 = store_thm(
-  "cbnf_of_works1",
-  ``(bnf_of M = SOME N) ⇒
-    cbnf_of @@ cDB (fromTerm M) -n->* cDB (fromTerm N)``,
-  SRW_TAC [][cbnf_of_def, bnf_of_def] THEN
-  IMP_RES_TAC cbnf_of_lemma THEN
-  ASM_SIMP_TAC (bsrw_ss()) [] THEN
-  ASM_SIMP_TAC (bsrw_ss()) [Once chap2Theory.lameq_Y] THEN
-  IMP_RES_TAC whileTheory.OWHILE_ENDCOND THEN
-  FULL_SIMP_TAC (srw_ss()) [] THEN
-  ASM_SIMP_TAC (bsrw_ss()) [cbnfof_body_equiv, cB_behaviour,
-                            cbnf_behaviour]);
 
 val FV_Yf = Store_thm(
   "FV_Yf",
@@ -1453,25 +1480,67 @@ val FV_Yf = Store_thm(
   SRW_TAC [boolSimps.CONJ_ss][chap2Theory.Yf_def, EXTENSION, LET_THM] THEN
   NEW_ELIM_TAC THEN METIS_TAC []);
 
+
+val cbnf_ofk_lemma = prove(
+  ``∀t. (OWHILE ((~) o bnf) (THE o noreduct) t0 = SOME t) ⇒
+        Y @@ (cbnfof_body @@ k) @@ cDB (fromTerm t0) ==
+          Y @@ (cbnfof_body @@ k) @@ cDB (fromTerm t)``,
+  HO_MATCH_MP_TAC whileTheory.OWHILE_INV_IND THEN SRW_TAC [][] THEN
+  ASM_SIMP_TAC (bsrw_ss()) [] THEN
+  ASM_SIMP_TAC (bsrw_ss()) [Once chap2Theory.lameq_Y] THEN
+  ASM_SIMP_TAC (bsrw_ss()) [cbnfof_body_equiv, cbnf_behaviour,
+                            cnoreduct_behaviour, cB_behaviour]);
+
+
+val cbnf_of_works1 = store_thm(
+  "cbnf_of_works1",
+  ``(bnf_of M = SOME N) ⇒
+    cbnf_ofk @@ c @@ cDB (fromTerm M) == c @@ cDB (fromTerm N)``,
+  SRW_TAC [][cbnf_ofk_def, bnf_of_def] THEN
+  IMP_RES_TAC cbnf_ofk_lemma THEN
+  ASM_SIMP_TAC (bsrw_ss()) [] THEN
+  ASM_SIMP_TAC (bsrw_ss()) [Once chap2Theory.lameq_Y] THEN
+  IMP_RES_TAC whileTheory.OWHILE_ENDCOND THEN
+  FULL_SIMP_TAC (srw_ss()) [] THEN
+  ASM_SIMP_TAC (bsrw_ss()) [cbnfof_body_equiv, cB_behaviour,
+                            cbnf_behaviour]);
+
+(*   SRW_TAC [][cbnf_ofk_def, bnf_of_def] THEN
+  ONCE_REWRITE_TAC [relationTheory.RTC_CASES_RTC_TWICE] THEN
+  Q.EXISTS_TAC `Y @@ (cbnfof_body @@ c) @@ cDB (fromTerm M)` THEN
+  CONJ_TAC THEN1
+    (MATCH_MP_TAC whead_norm_congL THEN SRW_TAC [][wh_B]) THEN
+*)
+
+
 (* proving the other direction is rather involved *)
 val cbnf_of_lemma1 = prove(
   ``t -n->* cDB M ∧ (FV t = {}) ⇒
-    Yf cbnfof_body @@ t -n->*
-      cB (dbnf M) @@ t @@ (Yf cbnfof_body @@ (cnoreduct @@ t))``,
+    Yf (cbnfof_body @@ k) @@ t -n->*
+      cB (dbnf M) @@ (k @@ t) @@ (Yf (cbnfof_body @@ k) @@ (cnoreduct @@ t))``,
   STRIP_TAC THEN
   REWRITE_TAC [Once relationTheory.RTC_CASES_RTC_TWICE] THEN
-  Q.EXISTS_TAC `cbnfof_body @@ Yf cbnfof_body @@ t` THEN
+  Q.EXISTS_TAC `cbnfof_body @@ k @@ Yf (cbnfof_body @@ k) @@ t` THEN
   CONJ_TAC THEN1
     METIS_TAC [relationTheory.RTC_SINGLE, head_reductionTheory.whY2,
                whead_norm_congL] THEN
   REWRITE_TAC [Once cbnfof_body_def] THEN
-  MATCH_MP_TAC RTC1 THEN
-  Q.EXISTS_TAC `LAM "t" (cbnf @@ VAR "t" @@ VAR "t" @@
-                         (Yf cbnfof_body @@ (cnoreduct @@ VAR "t"))) @@ t` THEN
+  MATCH_MP_TAC RTC1 THEN FRESH_TAC THEN SRW_TAC [][tpm_fresh] THEN
+  Q.EXISTS_TAC `LAM f (LAM t0 (cbnf @@ VAR t0 @@ (k @@ VAR t0) @@
+                         (VAR f @@ (cnoreduct @@ VAR t0))))
+                 @@ Yf (cbnfof_body @@ k)
+                 @@ t` THEN
   CONJ_TAC THEN1
     SRW_TAC [][normorder_rwts, lemma14b] THEN
   MATCH_MP_TAC RTC1 THEN
-  Q.EXISTS_TAC `cbnf @@ t @@ t @@ (Yf cbnfof_body @@ (cnoreduct @@ t))` THEN
+  Q.EXISTS_TAC `LAM t0 (cbnf @@ VAR t0 @@ (k @@ VAR t0)
+                             @@ (Yf (cbnfof_body @@ k)
+                                    @@ (cnoreduct @@ VAR t0))) @@ t` THEN
+  CONJ_TAC THEN1
+    SRW_TAC [][normorder_rwts, lemma14b] THEN
+  MATCH_MP_TAC RTC1 THEN
+  Q.EXISTS_TAC
+    `cbnf @@ t @@ (k @@ t) @@ (Yf (cbnfof_body @@ k) @@ (cnoreduct @@ t))` THEN
   CONJ_TAC THEN1
     SRW_TAC [][normorder_rwts, lemma14b] THEN
   MATCH_MP_TAC whead_norm_congL THEN
@@ -1480,53 +1549,55 @@ val cbnf_of_lemma1 = prove(
 
 val cbnfof_body_loops = prove(
   ``t -n->* cDB M ∧ (FV t = {}) ∧ ¬dbnf M ⇒
-    Yf cbnfof_body @@ t -n->* Yf cbnfof_body @@ (cnoreduct @@ t)``,
-  STRIP_TAC THEN IMP_RES_TAC cbnf_of_lemma1 THEN POP_ASSUM MP_TAC THEN
-  SRW_TAC [][] THEN
+    Yf (cbnfof_body @@ k) @@ t -n->*
+       Yf (cbnfof_body @@ k) @@ (cnoreduct @@ t)``,
+  STRIP_TAC THEN IMP_RES_TAC cbnf_of_lemma1 THEN
+  POP_ASSUM (MP_TAC o SPEC_ALL) THEN SRW_TAC [][] THEN
   ONCE_REWRITE_TAC [relationTheory.RTC_CASES_RTC_TWICE] THEN
   POP_ASSUM (fn th => EXISTS_TAC (rand (concl th)) THEN ASSUME_TAC th) THEN
   SRW_TAC [][cB_behaviour]);
 
 val cbnfof_body_finishes = prove(
-  ``t -n->* cDB M ∧ (FV t = {}) ∧ dbnf M ⇒ Yf cbnfof_body @@ t -n->* cDB M``,
-  STRIP_TAC THEN IMP_RES_TAC cbnf_of_lemma1 THEN POP_ASSUM MP_TAC THEN
-  SRW_TAC [][] THEN
+  ``t -n->* cDB M ∧ (FV t = {}) ∧ dbnf M ⇒
+    Yf (cbnfof_body @@ k) @@ t -n->* k @@ t``,
+  STRIP_TAC THEN IMP_RES_TAC cbnf_of_lemma1 THEN
+  POP_ASSUM (MP_TAC o SPEC_ALL) THEN SRW_TAC [][] THEN
   ONCE_REWRITE_TAC [relationTheory.RTC_CASES_RTC_TWICE] THEN
   POP_ASSUM (fn th => EXISTS_TAC (rand (concl th)) THEN ASSUME_TAC th) THEN
-  SRW_TAC [][] THEN ASM_SIMP_TAC (bsrw_ss()) [cB_behaviour]);
-
+  SRW_TAC [][] THEN
+  ASM_SIMP_TAC (srw_ss()) [cB_behaviour]);
 
 val cbnf_of_works2_lemma = prove(
   ``∀t t' M.
       (FV t = {}) ∧ t -n->* cDB M ∧
-      Yf cbnfof_body @@ t -n->* t' ∧ bnf t' ⇒
-      ∃M'. (t' = cDB M') ∧
-           (bnf_of (toTerm M) = SOME (toTerm M'))``,
-  completeInduct_on `THE (length (nopath (Yf cbnfof_body @@ t)))` THEN
+      Yf (cbnfof_body @@ k) @@ t -n->* t' ∧ bnf t' ⇒
+      ∃M'. (bnf_of (toTerm M) = SOME (toTerm M')) ∧
+           k @@ cDB M' -n->* t'``,
+  completeInduct_on `THE (length (nopath (Yf (cbnfof_body @@ k) @@ t)))` THEN
   FULL_SIMP_TAC (srw_ss() ++ boolSimps.DNF_ss) [] THEN
   REPEAT STRIP_TAC THEN
   Cases_on `dbnf M` THENL [
     Q.EXISTS_TAC `M` THEN IMP_RES_TAC cbnfof_body_finishes THEN
-    `cDB M -β->* t'` by METIS_TAC [bnf_triangle, nstar_betastar] THEN
-    `bnf (cDB M)` by SRW_TAC [][] THEN
-    `t' = cDB M` by METIS_TAC [bnf_reduction_to_self] THEN
-    SRW_TAC [][] THEN
+    `k @@ t -β->* t'` by METIS_TAC [bnf_triangle, nstar_betastar] THEN
+    `t' == k @@ t`
+       by METIS_TAC [betastar_lameq_bnf, chap2Theory.lam_eq_rules] THEN
+    ASM_SIMP_TAC (bsrw_ss()) [] THEN
     SRW_TAC [][bnf_of_def, Once whileTheory.OWHILE_THM],
     ALL_TAC
   ] THEN
-  IMP_RES_TAC cbnfof_body_loops THEN
-  `Yf cbnfof_body @@ (cnoreduct @@ t) -n->* t'`
+  IMP_RES_TAC cbnfof_body_loops THEN POP_ASSUM (ASSUME_TAC o SPEC_ALL) THEN
+  `Yf (cbnfof_body @@ k) @@ (cnoreduct @@ t) -n->* t'`
      by METIS_TAC [nstar_bnf_triangle] THEN
   `FV (cnoreduct @@ t) = {}` by SRW_TAC [][] THEN
   `cnoreduct @@ t -n->* cDB (fromTerm (THE (noreduct (toTerm M))))`
      by ASM_SIMP_TAC (bsrw_ss()) [cnoreduct_behaviour
                                     |> Q.SPEC `toTerm M`
                                     |> SIMP_RULE (srw_ss()) []] THEN
-  `Yf cbnfof_body @@ t ≠ Yf cbnfof_body @@ (cnoreduct @@ t)`
+  `Yf (cbnfof_body @@ k) @@ t ≠ Yf (cbnfof_body @@ k) @@ (cnoreduct @@ t)`
      by SRW_TAC [][APP_acyclic] THEN
-  `finite (nopath (Yf cbnfof_body @@ t))`
+  `finite (nopath (Yf (cbnfof_body @@ k) @@ t))`
      by METIS_TAC [has_bnf_thm, nstar_betastar, has_bnf_finite_nopath] THEN
-  FIRST_X_ASSUM (Q.SPECL_THEN [`cnoreduct @@ t`, `t'`,
+  FIRST_X_ASSUM (Q.SPECL_THEN [`k`, `cnoreduct @@ t`, `t'`,
                                `fromTerm (THE (noreduct (toTerm M)))`]
                               MP_TAC) THEN
   ASM_SIMP_TAC (srw_ss()) [] THEN
@@ -1538,33 +1609,48 @@ val cbnf_of_works2_lemma = prove(
   SRW_TAC [][bnf_of_def, Once whileTheory.OWHILE_THM] THEN
   SRW_TAC [][GSYM bnf_of_def]);
 
-val cbnf_of_works2 = store_thm(
-  "cbnf_of_works2",
-  ``cbnf_of @@ cDB M -n->* t' ∧ bnf t' ⇒
-    ∃M'. (t' = cDB M') ∧ (bnf_of (toTerm M) = SOME (toTerm M'))``,
+val cbnf_ofk_works2 = store_thm(
+  "cbnf_ofk_works2",
+  ``cbnf_ofk @@ k @@ cDB M -n->* t' ∧ bnf t' ⇒
+    ∃M'. (bnf_of (toTerm M) = SOME (toTerm M')) ∧ k @@ cDB M' -n->* t'``,
   STRIP_TAC THEN Q.PAT_ASSUM `XX -n->* YY` MP_TAC THEN
-  ASM_SIMP_TAC (bsrw_ss()) [cbnf_of_def,
+  ASM_SIMP_TAC (bsrw_ss()) [cbnf_ofk_def,
                             MATCH_MP relationTheory.RTC_SINGLE whY1] THEN
   STRIP_TAC THEN
-  `Yf cbnfof_body @@ cDB M -β->* t'`
+  `Yf (cbnfof_body @@ k) @@ cDB M -β->* t'`
      by METIS_TAC [betastar_lameq_bnf] THEN
-  `Yf cbnfof_body @@ cDB M -n->* t'`
+  `Yf (cbnfof_body @@ k) @@ cDB M -n->* t'`
      by METIS_TAC [nstar_betastar_bnf] THEN
   Q.SPECL_THEN [`cDB M`, `t'`, `M`] MP_TAC cbnf_of_works2_lemma THEN
-  SRW_TAC [][] THEN METIS_TAC []);
+  SRW_TAC [][] THEN METIS_TAC [nstar_lameq]);
+
+val bnfNONE_cbnf_ofk_fails = store_thm(
+  "bnfNONE_cbnf_ofk_fails",
+  ``(bnf_of M = NONE) ⇒ ¬has_bnf (cbnf_ofk @@ k @@ cDB (fromTerm M))``,
+  REPEAT STRIP_TAC THEN
+  `∃t'. cbnf_ofk @@ k @@ cDB (fromTerm M) -n->* t' ∧ bnf t'`
+     by METIS_TAC [has_bnf_thm, nstar_betastar_bnf] THEN
+  IMP_RES_TAC (REWRITE_RULE [GSYM AND_IMP_INTRO] cbnf_ofk_works2) THEN
+  FULL_SIMP_TAC (srw_ss()) []);
 
 val cbnf_of_fails = store_thm(
   "cbnf_of_fails",
   ``(bnf_of M = NONE) ⇔ ¬has_bnf (cbnf_of @@ cDB (fromTerm M))``,
-  EQ_TAC THEN STRIP_TAC THENL [
-    STRIP_TAC THEN
-    `∃t'. cbnf_of @@ cDB (fromTerm M) -n->* t' ∧ bnf t'`
-       by METIS_TAC [has_bnf_thm, nstar_betastar_bnf] THEN
-    IMP_RES_TAC (REWRITE_RULE [GSYM AND_IMP_INTRO] cbnf_of_works2) THEN
-    FULL_SIMP_TAC (srw_ss()) [],
+  SRW_TAC [][EQ_IMP_THM, bnfNONE_cbnf_ofk_fails, cbnf_of_def] THEN
+  Cases_on `bnf_of M` THEN SRW_TAC [][] THEN
+  IMP_RES_TAC cbnf_of_works1 THEN
+  `cbnf_ofk @@ I @@ cDB (fromTerm M) == cDB (fromTerm x)`
+    by METIS_TAC [chap2Theory.lam_eq_rules, chap2Theory.lameq_I] THEN
+  METIS_TAC [bnf_cDB, betastar_lameq_bnf, has_bnf_thm]);
 
-    Cases_on `bnf_of M` THEN SRW_TAC [][] THEN
-    METIS_TAC [cbnf_of_works1, bnf_cDB, nstar_betastar_bnf, has_bnf_thm]
-  ]);
+val cbnf_force_num_fails = store_thm(
+  "cbnf_force_num_fails",
+  ``¬has_bnf (cbnf_ofk @@ cforce_num @@ cDB (fromTerm M)) ⇒
+    (bnf_of M = NONE)``,
+  REPEAT STRIP_TAC THEN Cases_on `bnf_of M` THEN SRW_TAC [][] THEN
+  IMP_RES_TAC cbnf_of_works1 THEN
+  POP_ASSUM (Q.SPEC_THEN `cforce_num` MP_TAC) THEN
+  SIMP_TAC (bsrw_ss()) [cforce_num_behaviour] THEN
+  METIS_TAC [bnf_church, betastar_lameq_bnf, has_bnf_thm]);
 
 val _ = export_theory()
